formal/SAL-examples/Drinks_Machine_LTL.thy
@@ -2,20 +2,67 @@ theory Drinks_Machine_LTL
 imports "../examples/Drinks_Machine" EFSM_LTL
 begin
 
+declare One_nat_def [simp del]
+
+lemma LTL_r2_not_always_gt_100: "not (alw (checkInx rg 2 ValueGt (Some (Num 100)))) (watch drinks i)"
+  apply (simp add: not_alw_iff watch_def)
+  apply (rule ev.base)
+  by (simp add: ValueGt_def)
+
+lemma apply_updates_select: "length b = 1 \<Longrightarrow> EFSM.apply_updates (Updates select) (case_vname (\<lambda>n. input2state b 1 (I n)) Map.empty) Map.empty = <R 1 := hd b, R 2 := Num 0>"
+  apply (rule ext)
+  by (simp add: select_def hd_input2state)
+
+lemma possible_steps_select_wrong_arity: "a = STR ''select'' \<Longrightarrow>
+       length b \<noteq> 1 \<Longrightarrow>
+       possible_steps drinks 0 Map.empty a b = {||}"
+  apply (simp add: possible_steps_def ffilter_def fset_both_sides Abs_fset_inverse Set.filter_def drinks_def)
+  apply safe
+  by (simp_all add: select_def)
+
+lemma possible_steps_0_not_select: "a \<noteq> STR ''select'' \<Longrightarrow>
+       possible_steps drinks 0 Map.empty a b = {||}"
+  apply (simp add: possible_steps_def ffilter_def fset_both_sides Abs_fset_inverse Set.filter_def drinks_def)
+  apply safe
+  by (simp_all add: select_def)
+
+lemma LTL_nxt_2_means_vend: "alw (nxt (StateEq (Some 2)) impl (StateEq (Some 1))) (watch drinks i)"
+proof(coinduction)
+  case alw
+  then show ?case
+    apply (simp add: watch_def)
+    apply (case_tac "shd i")
+    apply simp
+    apply (case_tac "a = STR ''select''")
+     apply (case_tac "length b = 1")
+      apply (simp add: possible_steps_0 apply_updates_select)
+      defer
+      apply (simp add: possible_steps_select_wrong_arity)
+      apply (metis (no_types, lifting) once_none_always_none StateEq_def alw.cases alw.coinduct option.distinct(1))
+     apply (simp add: possible_steps_0_not_select)
+     apply (metis (no_types, lifting) once_none_always_none StateEq_def alw.cases alw.coinduct option.distinct(1))
+    apply standard
+     apply (simp add: StateEq_def)
+    apply (rule disjI2)
+    oops
+
+lemma LTL_costsMoney_aux: "(alw ((not (checkInx rg 2 ValueGt (Some (Num 100)))) impl (not (nxt (StateEq (Some 2)))))) (watch drinks i)"
+  oops
+
   (* costsMoney: THEOREM drinks |- G(X(cfstate=State_2) => gval(value_ge(r_2, Some(NUM(100))))); *)
-lemma costsMoney: "alw(nxt(StateEq (Some 2)) impl (checkInx rg 2 ValueGt (Some (Num 100)))) (watch drinks i)"
+lemma LTL_costsMoney: "(alw ((nxt (StateEq (Some 2))) impl ((checkInx rg 2 ValueGt (Some (Num 100)))))) (watch drinks i)"
   oops
 
 (* neverReachS2: THEOREM drinks |- label=select AND I(1) = STR(String_coke) AND
                                 X(label=coin AND I(1) = NUM(100)) AND
                                 X(X(label=vend AND I=InputSequence !empty)) => X(X(X(cfstate=State_2)));;*)
-lemma neverReachS2:"(((((LabelEq ''select'') aand (checkInx ip 1 ValueEq (Some (Str ''coke''))))
+lemma LTL_neverReachS2:"(((((LabelEq ''select'') aand (checkInx ip 1 ValueEq (Some (Str ''coke''))))
                     aand
                     (nxt ((LabelEq ''coin'') aand (checkInx ip 1 ValueEq (Some (Num 100))))))
                     aand
-                    (nxt(nxt((LabelEq ''vend'' aand (InputEq []))))))
+                    (nxt (nxt((LabelEq ''vend'' aand (InputEq []))))))
                     impl
-                    (nxt(nxt (nxt (StateEq (Some 2))))))
+                    (nxt (nxt (nxt (StateEq (Some 2))))))
                     (watch drinks i)"
   oops
 
